Semantics.thy
@@ -4,13 +4,14 @@ text\<open>For next meeting:
 Questions/Help:
 - Nominal2 proof for lookup_instance. Can't get the first goal to be solved.
   Figured it was more productive to keep going for now.
+- See free_constructors packet below.
 - Heaps, see text block below.
 To talk about:
 - Think I figured out what's going on with expression and formula semantics, see below.
 - See TODOs on the exp small-step semantics.
 - See TODO on exp.\<close>
 
-datatype headers = Instances "instanc \<Rightarrow> bv option"
+datatype headers = Headers "instanc \<Rightarrow> bv option"
 datatype heap = Heap bv bv headers
 
 text\<open>This is necessary to use heaps in nominal_functions. It basically states that
@@ -26,17 +27,25 @@ instantiation heap :: pure begin
   instance by standard (auto simp add: permute_heap_def)
 end
 
+free_constructors packet for PktIn | PktOut
+using packet.strong_exhaust apply auto done
+(* TODO: Are these warnings bad? Can I do something about them? *)
+(* TODO: Is it preferable to do this, or make every function matching on packets
+         a nominal_function? *)
+(* TODO: This works when done here but not when done in Syntax? *)
+
 fun triple_to_heap :: "bv \<Rightarrow> bv \<Rightarrow> headers \<Rightarrow> heap" where
   "triple_to_heap In Out H = Heap In Out H"
 
-(* doesn't work because of nominal_datatype vs datatype right now I think.
-   But Dmitriy had some way of making these constructors? *)
+fun header_lookup :: "headers \<Rightarrow> instanc \<Rightarrow> bv option" where
+  "header_lookup (Headers h) i = h i" 
+
 fun heap_lookup_packet :: "heap \<Rightarrow> packet \<Rightarrow> bv" where
   "heap_lookup_packet (Heap In Out _) PktIn = In" |
-  "heap_lookup_packet (Heap In Out _) PktOut = Out" 
+  "heap_lookup_packet (Heap In Out _) PktOut = Out"
 
 fun heap_lookup_instance :: "heap \<Rightarrow> instanc \<Rightarrow> bv option" where
-  "heap_lookup_instance (Heap _ (Instances insts)) i = insts i"
+  "heap_lookup_instance (Heap _ _ (Headers insts)) i = insts i"
 
 (* Easier to work with than "var \<Rightarrow> heap" with Nominal2 because it has a finite support (I think) *)
 type_synonym env = "(var \<times> heap) list"
@@ -46,13 +55,13 @@ declare
   fresh_star_Pair[simp] fresh_star_insert[simp] fresh_Nil[simp]
   pure_supp[simp] pure_fresh[simp]
 
-fun lookup_packet :: "env \<Rightarrow> var \<Rightarrow> packet \<Rightarrow> bv option" where
-  "lookup_packet \<epsilon> x p = map_option (\<lambda>h. heap_lookup_packet h p) (map_of \<epsilon> x)"
-fun lookup_instance :: "env \<Rightarrow> var \<Rightarrow> instanc \<Rightarrow> bv option" where
-  "lookup_instance \<epsilon> x i = Option.bind (map_of \<epsilon> x) (\<lambda>h. heap_lookup_instance h i)"
-nominal_function lookup_sliceable :: "sliceable \<Rightarrow> env \<Rightarrow> bv option" where
-  "lookup_sliceable (SlPacket x p) \<epsilon> = lookup_packet \<epsilon> x p" |
-  "lookup_sliceable (SlInstance x i) \<epsilon> = lookup_instance \<epsilon> x i"
+fun env_lookup_packet :: "env \<Rightarrow> var \<Rightarrow> packet \<Rightarrow> bv option" where
+  "env_lookup_packet \<epsilon> x p = map_option (\<lambda>h. heap_lookup_packet h p) (map_of \<epsilon> x)"
+fun env_lookup_instance :: "env \<Rightarrow> var \<Rightarrow> instanc \<Rightarrow> bv option" where
+  "env_lookup_instance \<epsilon> x i = Option.bind (map_of \<epsilon> x) (\<lambda>h. heap_lookup_instance h i)"
+nominal_function env_lookup_sliceable :: "env \<Rightarrow> sliceable \<Rightarrow> bv option" where
+  "env_lookup_sliceable \<epsilon> (SlPacket x p) = env_lookup_packet \<epsilon> x p" |
+  "env_lookup_sliceable \<epsilon> (SlInstance x i) = env_lookup_instance \<epsilon> x i"
 sorry
 (*  using [[simproc del: alpha_lst defined_all]]
   subgoal by (simp add: eqvt_def lookup_sliceable_graph_aux_def)
@@ -72,11 +81,10 @@ sorry
 nominal_termination (eqvt)
   by lexicographic_order
 
-term lookup_sliceable_graph_aux
-
 fun slice :: "'a list \<Rightarrow> int \<Rightarrow> int \<Rightarrow> 'a list" where
   "slice xs n m = take (nat (m - n)) (drop (nat n) xs)"
 
+section\<open>Expressions and Formulas\<close>
 
 text\<open>About the semantics for expressions and formulas...
 The paper references, but never defines, small-step semantics for formulas and expressions, which
@@ -118,67 +126,117 @@ have the HT that gives us types for each instanc, so can just look up the range 
 name.
 \<close>
 
+subsection\<open>Small-step semantics\<close>
+
 (* TODO: At the moment, we just ignore variables here and assume they must be "heap". Should we
-   explicitly encode that in the rule assumptions? *)
+   explicitly encode that somehow, perhaps in the rule assumptions? *)
 (* TODO: Which of these is preferable?
     E_PktIn:      "(In, Out, H, Packet x PktIn) \<rightarrow> Bv In" |
     E_PktIn:      "\<lbrakk> p = PktIn \<rbrakk> \<Longrightarrow> (In, Out, H, Packet x p) \<rightarrow> Bv In" |
   and similarly, keep len call in the rule or make it a premise in E_Pkt*Len?
 *)
 inductive
-  exp_small_step :: "(bv \<times> bv \<times> headers \<times> exp) \<Rightarrow> exp \<Rightarrow> bool" ("_ \<rightarrow>/ _" [0,50] 50)
+  exp_small_step :: "(bv \<times> bv \<times> headers \<times> exp) \<Rightarrow> exp \<Rightarrow> bool" ("_ \<rightarrow>\<^sub>e _" [0,50] 50)
 where
-  E_Plus1:      "\<lbrakk> (In, Out, H, e\<^sub>1) \<rightarrow> e\<^sub>1' \<rbrakk>
-                \<Longrightarrow> (In, Out, H, Plus e\<^sub>1 e\<^sub>2) \<rightarrow> Plus e\<^sub>1' e\<^sub>2" |
-  E_Plus2:      "\<lbrakk> value v\<^sub>1; (In, Out, H, e\<^sub>2) \<rightarrow> e\<^sub>2' \<rbrakk>
-                \<Longrightarrow> (In, Out, H, Plus v\<^sub>1 e\<^sub>2) \<rightarrow> Plus v\<^sub>1 e\<^sub>2'" |
+  E_Plus1:      "\<lbrakk> (In, Out, H, e\<^sub>1) \<rightarrow>\<^sub>e e\<^sub>1' \<rbrakk>
+                \<Longrightarrow> (In, Out, H, Plus e\<^sub>1 e\<^sub>2) \<rightarrow>\<^sub>e Plus e\<^sub>1' e\<^sub>2" |
+  E_Plus2:      "\<lbrakk> value\<^sub>e v\<^sub>1; (In, Out, H, e\<^sub>2) \<rightarrow>\<^sub>e e\<^sub>2' \<rbrakk>
+                \<Longrightarrow> (In, Out, H, Plus v\<^sub>1 e\<^sub>2) \<rightarrow>\<^sub>e Plus v\<^sub>1 e\<^sub>2'" |
   E_Plus:       "\<lbrakk> v\<^sub>1 = Num n\<^sub>1; v\<^sub>2 = Num n\<^sub>2 \<rbrakk>
-                \<Longrightarrow> (In, Out, H, Plus v\<^sub>1 v\<^sub>2) \<rightarrow> Num (n\<^sub>1 + n\<^sub>2)" |
-  E_Concat1:    "\<lbrakk> (In, Out, H, e\<^sub>1) \<rightarrow> e\<^sub>1' \<rbrakk>
-                \<Longrightarrow> (In, Out, H, Concat e\<^sub>1 e\<^sub>2) \<rightarrow> Concat e\<^sub>1 e\<^sub>2" |
-  E_Concat2:    "\<lbrakk> value v\<^sub>1; (In, Out, H, e\<^sub>2) \<rightarrow> e\<^sub>2' \<rbrakk>
-                \<Longrightarrow> (In, Out, H, Concat v\<^sub>1 e\<^sub>2) \<rightarrow> Concat v\<^sub>1 e\<^sub>2'" |
+                \<Longrightarrow> (In, Out, H, Plus v\<^sub>1 v\<^sub>2) \<rightarrow>\<^sub>e Num (n\<^sub>1 + n\<^sub>2)" |
+  E_Concat1:    "\<lbrakk> (In, Out, H, e\<^sub>1) \<rightarrow>\<^sub>e e\<^sub>1' \<rbrakk>
+                \<Longrightarrow> (In, Out, H, Concat e\<^sub>1 e\<^sub>2) \<rightarrow>\<^sub>e Concat e\<^sub>1 e\<^sub>2" |
+  E_Concat2:    "\<lbrakk> value\<^sub>e v\<^sub>1; (In, Out, H, e\<^sub>2) \<rightarrow>\<^sub>e e\<^sub>2' \<rbrakk>
+                \<Longrightarrow> (In, Out, H, Concat v\<^sub>1 e\<^sub>2) \<rightarrow>\<^sub>e Concat v\<^sub>1 e\<^sub>2'" |
   E_Concat:     "\<lbrakk> v\<^sub>1 = Bv b\<^sub>1; v\<^sub>2 = Bv b\<^sub>2 \<rbrakk>
-                \<Longrightarrow> (In, Out, H, Concat v\<^sub>1 v\<^sub>2) \<rightarrow> Bv (b\<^sub>1 @ b\<^sub>2)" |
-  E_PktIn:      "(In, Out, H, Packet x PktIn) \<rightarrow> Bv In" |
-  E_PktOut:     "(In, Out, H, Packet x PktOut) \<rightarrow> Bv Out" |
-  E_PktInLen:   "(In, Out, H, Len x PktIn) \<rightarrow> Num (len In)" |
-  E_PktOutLen:  "(In, Out, H, Len x PktOut) \<rightarrow> Num (len Out)" |
-  (*E_Slice1:     "\<lbrakk> (In, Out, H, e\<^sub>1) \<rightarrow> e\<^sub>1' \<rbrakk>
-                \<Longrightarrow> (In, Out, H, Slice sl e\<^sub>1 e\<^sub>2) \<rightarrow> Slice sl e\<^sub>1' e\<^sub>2" |
-  E_Slice2:     "\<lbrakk> value v\<^sub>1; (In, Out, H, e\<^sub>2) \<rightarrow> e\<^sub>2' \<rbrakk>
-                \<Longrightarrow> (In, Out, H, Slice sl v\<^sub>1 e\<^sub>2) \<rightarrow> Slice sl v\<^sub>1 e\<^sub>2'" | *)
+                \<Longrightarrow> (In, Out, H, Concat v\<^sub>1 v\<^sub>2) \<rightarrow>\<^sub>e Bv (b\<^sub>1 @ b\<^sub>2)" |
+  E_PktIn:      "(In, Out, H, Packet x PktIn) \<rightarrow>\<^sub>e Bv In" |
+  E_PktOut:     "(In, Out, H, Packet x PktOut) \<rightarrow>\<^sub>e Bv Out" |
+  E_PktInLen:   "(In, Out, H, Len x PktIn) \<rightarrow>\<^sub>e Num (len In)" |
+  E_PktOutLen:  "(In, Out, H, Len x PktOut) \<rightarrow>\<^sub>e Num (len Out)" |
+  (*E_Slice1:     "\<lbrakk> (In, Out, H, e\<^sub>1) \<rightarrow>\<^sub>e e\<^sub>1' \<rbrakk>
+                \<Longrightarrow> (In, Out, H, Slice sl e\<^sub>1 e\<^sub>2) \<rightarrow>\<^sub>e Slice sl e\<^sub>1' e\<^sub>2" |
+  E_Slice2:     "\<lbrakk> value\<^sub>e v\<^sub>1; (In, Out, H, e\<^sub>2) \<rightarrow>\<^sub>e e\<^sub>2' \<rbrakk>
+                \<Longrightarrow> (In, Out, H, Slice sl v\<^sub>1 e\<^sub>2) \<rightarrow>\<^sub>e Slice sl v\<^sub>1 e\<^sub>2'" | *)
   E_SlicePktIn: "\<lbrakk> 0 \<le> n \<and> n < m \<and> m \<le> (len In + 1); slice In n m = bs \<rbrakk>
-                \<Longrightarrow> (In, Out, H, Slice (SlPacket x PktIn) n m) \<rightarrow> Bv bs" |
+                \<Longrightarrow> (In, Out, H, Slice (SlPacket x PktIn) n m) \<rightarrow>\<^sub>e Bv bs" |
   E_SlicePktOut:"\<lbrakk> 0 \<le> n \<and> n < m \<and> m \<le> (len Out + 1); slice Out n m = bs \<rbrakk>
-                \<Longrightarrow> (In, Out, H, Slice (SlPacket x PktOut) n m) \<rightarrow> Bv bs" |
-  E_SliceInst:  "\<lbrakk> H \<rbrakk>
-                \<Longrightarrow> (In, Out, H, Slice (SlInstance x i) n m) \<rightarrow> Num 0"
+                \<Longrightarrow> (In, Out, H, Slice (SlPacket x PktOut) n m) \<rightarrow>\<^sub>e Bv bs" |
+  E_SliceInst:  "\<lbrakk> header_lookup H i = Some bv; 0 \<le> n \<and> n < m \<and> m \<le> (len bv + 1); slice bv n m = bs \<rbrakk>
+                \<Longrightarrow> (In, Out, H, Slice (SlInstance x i) n m) \<rightarrow>\<^sub>e Bv bs"
 
-inductive exp_sem :: "exp \<Rightarrow> env \<Rightarrow> val \<Rightarrow> bool" where
-  "exp_sem (Syntax.Num n) _ (Num n)" |
-  "exp_sem (Bv bs) _ (BV bs)" |
-  "\<lbrakk> lookup_packet \<epsilon> x p = Some bs; len bs = n \<rbrakk> \<Longrightarrow> exp_sem (Len x p) \<epsilon> (Num n)" |
-  "\<lbrakk> exp_sem e\<^sub>1 \<epsilon> (Num n\<^sub>1); exp_sem e\<^sub>2 \<epsilon> (Num n\<^sub>2) \<rbrakk> \<Longrightarrow> exp_sem (Plus e\<^sub>1 e\<^sub>2) \<epsilon> (Num (n\<^sub>1 + n\<^sub>2))" |
-  "\<lbrakk> exp_sem e\<^sub>1 \<epsilon> (BV b\<^sub>1); exp_sem e\<^sub>2 \<epsilon> (BV b\<^sub>2) \<rbrakk> \<Longrightarrow> exp_sem (Concat e\<^sub>1 e\<^sub>2) \<epsilon> (BV (b\<^sub>1 @ b\<^sub>2))" |
-  "\<lbrakk> lookup_packet \<epsilon> x p = Some bs \<rbrakk> \<Longrightarrow> exp_sem (Packet x p) \<epsilon> (BV bs)" |
-  "\<lbrakk> lookup_packet \<epsilon> x p = Some bs;  0 \<le> n \<and> n < m \<and> m \<le> (len bs + 1); slice bs n m = bs' \<rbrakk>
-    \<Longrightarrow> exp_sem (Slice (SlPacket x p) n m) \<epsilon> (BV bs')"
+inductive formula_small_step :: "(bv \<times> bv \<times> headers \<times> formula) \<Rightarrow> formula \<Rightarrow> bool" ("_ \<rightarrow>\<^sub>f _" [0,50] 50)
+where
+  F_Eq1:        "\<lbrakk> (In, Out, H, e\<^sub>1) \<rightarrow>\<^sub>e e\<^sub>1' \<rbrakk>
+                \<Longrightarrow> (In, Out, H, Eq e\<^sub>1 e\<^sub>2) \<rightarrow>\<^sub>f Eq e\<^sub>1' e\<^sub>2" |
+  F_Eq2:        "\<lbrakk> value\<^sub>e v\<^sub>1; (In, Out, H, e\<^sub>2) \<rightarrow>\<^sub>e e\<^sub>2' \<rbrakk>
+                \<Longrightarrow> (In, Out, H, Eq v\<^sub>1 e\<^sub>2) \<rightarrow>\<^sub>f Eq v\<^sub>1 e\<^sub>2'" |
+  F_EqTrue:     "\<lbrakk> value\<^sub>e v\<^sub>1; value\<^sub>e v\<^sub>2; v\<^sub>1 = v\<^sub>2 \<rbrakk>
+                \<Longrightarrow> (In, Out, H, Eq v\<^sub>1 v\<^sub>2) \<rightarrow>\<^sub>f FTrue" |
+  F_EqFalse:    "\<lbrakk> value\<^sub>e v\<^sub>1; value\<^sub>e v\<^sub>2; v\<^sub>1 \<noteq> v\<^sub>2 \<rbrakk>
+                \<Longrightarrow> (In, Out, H, Eq v\<^sub>1 v\<^sub>2) \<rightarrow>\<^sub>f FFalse" |
+  F_Gt1:        "\<lbrakk> (In, Out, H, e\<^sub>1) \<rightarrow>\<^sub>e e\<^sub>1' \<rbrakk>
+                \<Longrightarrow> (In, Out, H, Gt e\<^sub>1 e\<^sub>2) \<rightarrow>\<^sub>f Gt e\<^sub>1' e\<^sub>2" |
+  F_Gt2:        "\<lbrakk> value\<^sub>e v\<^sub>1; (In, Out, H, e\<^sub>2) \<rightarrow>\<^sub>e e\<^sub>2' \<rbrakk>
+                \<Longrightarrow> (In, Out, H, Gt v\<^sub>1 e\<^sub>2) \<rightarrow>\<^sub>f Gt v\<^sub>1 e\<^sub>2'" |
+  F_GtTrue:     "\<lbrakk> v\<^sub>1 = Num n\<^sub>1; v\<^sub>2 = Num n\<^sub>2; n\<^sub>1 > n\<^sub>2 \<rbrakk>
+                \<Longrightarrow> (In, Out, H, Gt v\<^sub>1 v\<^sub>2) \<rightarrow>\<^sub>f FTrue" |
+  F_GtFalse:    "\<lbrakk> v\<^sub>1 = Num n\<^sub>1; v\<^sub>2 = Num n\<^sub>2; n\<^sub>1 \<le> n\<^sub>2 \<rbrakk>
+                \<Longrightarrow> (In, Out, H, Gt v\<^sub>1 v\<^sub>2) \<rightarrow>\<^sub>f FFalse" |
+  F_And1:       "\<lbrakk> (In, Out, H, f\<^sub>1) \<rightarrow>\<^sub>f f\<^sub>1' \<rbrakk>
+                \<Longrightarrow> (In, Out, H, And f\<^sub>1 f\<^sub>2) \<rightarrow>\<^sub>f And f\<^sub>1' f\<^sub>2" |
+  F_AndTrue:    "\<lbrakk> t\<^sub>1 = FTrue \<rbrakk>
+                \<Longrightarrow> (In, Out, H, And t\<^sub>1 f\<^sub>2) \<rightarrow>\<^sub>f f\<^sub>2" |
+  F_AndFalse:   "\<lbrakk> t\<^sub>1 = FFalse \<rbrakk>
+                \<Longrightarrow> (In, Out, H, And t\<^sub>1 f\<^sub>2) \<rightarrow>\<^sub>f FFalse" |
+  F_Not1:       "\<lbrakk> (In, Out, H, f\<^sub>1) \<rightarrow>\<^sub>f f\<^sub>1' \<rbrakk>
+                \<Longrightarrow> (In, Out, H, Not f\<^sub>1) \<rightarrow>\<^sub>f f\<^sub>1'" |
+  F_NotTrue:    "\<lbrakk> t\<^sub>1 = FTrue \<rbrakk>
+                \<Longrightarrow> (In, Out, H, Not t\<^sub>1) \<rightarrow>\<^sub>f FFalse" |
+  F_NotFalse:   "\<lbrakk> t\<^sub>1 = FFalse \<rbrakk>
+                \<Longrightarrow> (In, Out, H, Not t\<^sub>1) \<rightarrow>\<^sub>f FTrue" |
+  F_IsValidTrue:"\<lbrakk> header_lookup H i = Some _ \<rbrakk>
+                \<Longrightarrow> (In, Out, H, IsValid x i) \<rightarrow>\<^sub>f FTrue" |
+  F_IsValidFalse:"\<lbrakk> header_lookup H i = None \<rbrakk>
+                \<Longrightarrow> (In, Out, H, IsValid x i) \<rightarrow>\<^sub>f FFalse"
 
-(* Should I make these small-step instead? Both form_sem and exp_sem *)
+subsection\<open>Denotational semantics\<close>
 
-inductive form_sem :: "formula \<Rightarrow> env \<Rightarrow> bool \<Rightarrow> bool" where
-  "\<lbrakk> exp_sem e\<^sub>1 \<epsilon> v; exp_sem e\<^sub>2 \<epsilon> v \<rbrakk> \<Longrightarrow> form_sem (Eq e\<^sub>1 e\<^sub>2) \<epsilon> true" |
-  "\<lbrakk> exp_sem e\<^sub>1 \<epsilon> v\<^sub>1; exp_sem e\<^sub>2 \<epsilon> v\<^sub>2; v\<^sub>1 \<noteq> v\<^sub>2 \<rbrakk> \<Longrightarrow> form_sem (Eq e\<^sub>1 e\<^sub>2) \<epsilon> false" |
-  "\<lbrakk> exp_sem e\<^sub>1 \<epsilon> (Num n\<^sub>1); exp_sem e\<^sub>2 \<epsilon> (Num n\<^sub>2); n\<^sub>1 > n\<^sub>2 \<rbrakk> \<Longrightarrow> form_sem (Gt e\<^sub>1 e\<^sub>2) \<epsilon> true" |
-  "\<lbrakk> exp_sem e\<^sub>1 \<epsilon> (Num n\<^sub>1); exp_sem e\<^sub>2 \<epsilon> (Num n\<^sub>2); n\<^sub>1 \<le> n\<^sub>2 \<rbrakk> \<Longrightarrow> form_sem (Gt e\<^sub>1 e\<^sub>2) \<epsilon> false"
-  (*"\<lbrakk> exp_sem e\<^sub>1 \<epsilon> (Num n\<^sub>1); exp_sem e\<^sub>2 \<epsilon> (Num n\<^sub>2); n\<^sub>1 \<le> n\<^sub>2 \<rbrakk> \<Longrightarrow> form_sem (And e\<^sub>1 e\<^sub>2) \<epsilon> false"*)
+nominal_function exp_sem :: "exp \<Rightarrow> env \<Rightarrow> val option" ("\<lbrakk>_ in _\<rbrakk>\<^sub>e" [50,60] 50)
+where
+  "\<lbrakk>Num n in \<epsilon>\<rbrakk>\<^sub>e = Some (VNum n)" |
+  "\<lbrakk>Bv bv in \<epsilon>\<rbrakk>\<^sub>e = Some (VBv bv)" |
+  "\<lbrakk>Plus e\<^sub>1 e\<^sub>2 in \<epsilon>\<rbrakk>\<^sub>e = (case (\<lbrakk>e\<^sub>1 in \<epsilon>\<rbrakk>\<^sub>e, \<lbrakk>e\<^sub>2 in \<epsilon>\<rbrakk>\<^sub>e) of
+    (Some (VNum n\<^sub>1), Some (VNum n\<^sub>2)) \<Rightarrow> Some (VNum (n\<^sub>1 + n\<^sub>2)) | _ \<Rightarrow> None)" |
+  "\<lbrakk>Concat e\<^sub>1 e\<^sub>2 in \<epsilon>\<rbrakk>\<^sub>e = (case (\<lbrakk>e\<^sub>1 in \<epsilon>\<rbrakk>\<^sub>e, \<lbrakk>e\<^sub>2 in \<epsilon>\<rbrakk>\<^sub>e) of
+    (Some (VBv bv\<^sub>1), Some (VBv bv\<^sub>2)) \<Rightarrow> Some (VBv (bv\<^sub>1 @ bv\<^sub>2)) | _ \<Rightarrow> None)" |
+  "\<lbrakk>Packet x p in \<epsilon>\<rbrakk>\<^sub>e = map_option (\<lambda>bv. VBv bv) (env_lookup_packet \<epsilon> x p)" |
+  "\<lbrakk>Len x p in \<epsilon>\<rbrakk>\<^sub>e = map_option (\<lambda>bv. VNum (len bv)) (env_lookup_packet \<epsilon> x p)" |
+  "\<lbrakk>Slice sl n m in \<epsilon>\<rbrakk>\<^sub>e = Option.bind (env_lookup_sliceable \<epsilon> sl)
+    (\<lambda>bv. if 0 \<le> n \<and> n < m \<and> m \<le> (len bv + 1) then Some (VBv (slice bv n m)) else None)"
+sorry
 
-(*datatype cmd =
-  Extract instanc | Remit instanc | Add instanc |
-  If formula cmd cmd | Seq cmd cmd | Assign instanc string exp |
-  Skip | Reset | Ascribe cmd pi_ty
-*)
+nominal_termination (eqvt)
+  by lexicographic_order
+
+nominal_function formula_sem :: "formula \<Rightarrow> env \<Rightarrow> bool option" ("\<lbrakk>_ in _\<rbrakk>\<^sub>f" [50,60] 50)
+where
+  "\<lbrakk>FTrue in \<epsilon>\<rbrakk>\<^sub>f = Some True" |
+  "\<lbrakk>FFalse in \<epsilon>\<rbrakk>\<^sub>f = Some False" |
+  "\<lbrakk>Eq e\<^sub>1 e\<^sub>2 in \<epsilon>\<rbrakk>\<^sub>f = (case (\<lbrakk>e\<^sub>1 in \<epsilon>\<rbrakk>\<^sub>e, \<lbrakk>e\<^sub>2 in \<epsilon>\<rbrakk>\<^sub>e) of
+    (Some v\<^sub>1, Some v\<^sub>2) \<Rightarrow> Some (v\<^sub>1 = v\<^sub>2) | _ \<Rightarrow> None)" |
+  "\<lbrakk>Gt e\<^sub>1 e\<^sub>2 in \<epsilon>\<rbrakk>\<^sub>f = (case (\<lbrakk>e\<^sub>1 in \<epsilon>\<rbrakk>\<^sub>e, \<lbrakk>e\<^sub>2 in \<epsilon>\<rbrakk>\<^sub>e) of
+    (Some (VNum n\<^sub>1), Some (VNum n\<^sub>2)) \<Rightarrow> Some (n\<^sub>1 > n\<^sub>2) | _ \<Rightarrow> None)" |
+  "\<lbrakk>And f\<^sub>1 f\<^sub>2 in \<epsilon>\<rbrakk>\<^sub>f = (case \<lbrakk>f\<^sub>1 in \<epsilon>\<rbrakk>\<^sub>f of None \<Rightarrow> None | Some False \<Rightarrow> Some False |
+    Some True \<Rightarrow> \<lbrakk>f\<^sub>2 in \<epsilon>\<rbrakk>\<^sub>f)" |
+  "\<lbrakk>Not f\<^sub>1 in \<epsilon>\<rbrakk>\<^sub>f = map_option (\<lambda>b. \<not>b) (\<lbrakk>f\<^sub>1 in \<epsilon>\<rbrakk>\<^sub>f)" |
+  "\<lbrakk>IsValid x i in \<epsilon>\<rbrakk>\<^sub>f = map_option (\<lambda>bv. True) (env_lookup_instance \<epsilon> x i)"
+sorry
+
+nominal_termination (eqvt)
+  by lexicographic_order
+
+section\<open>Commands\<close>
 
 (* I added HT as the extra ambient/global context explicitly here. *)
 inductive
